tests/lean/run/linearByRefl.lean
@@ -1,253 +1,48 @@
-abbrev Var := Nat
-
-inductive Expr where
-  | num  (v : Nat)
-  | var  (i : Var)
-  | add  (a b : Expr)
-  | mulL (k : Nat) (a : Expr)
-  | mulR (a : Expr) (k : Nat)
-  deriving Inhabited, Repr
-
-structure Context where
-  vars : List Nat
-
-def List.getIdx : List α → Var → α → α
-  | [],    i,   u => u
-  | a::as, 0,   u => a
-  | a::as, i+1, u => getIdx as i u
-
-def Var.denote (ctx : Context) (v : Var) : Nat :=
-  ctx.vars.getIdx v 0
-
-def Expr.denote (ctx : Context) : Expr → Nat
-  | Expr.add a b  => Nat.add (denote ctx a) (denote ctx b)
-  | Expr.num k    => k
-  | Expr.var v    => v.denote ctx
-  | Expr.mulL k e => k * denote ctx e
-  | Expr.mulR e k => denote ctx e * k
-
-abbrev Monomials := List (Nat × Var)
-
-def Monomials.denote (ctx : Context) (m : Monomials) : Nat :=
-  match m with
-  | [] => 0
-  | (k, v) :: m => k * v.denote ctx + denote ctx m
-
-def Monomials.addM (m : Monomials) (k : Nat) (v : Var) : Monomials :=
-  match m with
-  | [] => [(k, v)]
-  | (k', v') :: m => if v = v' then (k' + k, v) :: m else (k', v') :: addM m k v
-
-attribute [local simp] Nat.add_comm Nat.add_assoc Nat.add_left_comm Nat.right_distrib Nat.left_distrib Nat.mul_assoc Nat.mul_comm
-
-@[simp] theorem Monomials.denote_addM (ctx : Context) (m : Monomials) (k : Nat) (v : Var) : (m.addM k v).denote ctx = m.denote ctx + k * v.denote ctx := by
-  induction m with
-  | nil => simp [denote]
-  | cons kv m ih => cases kv with | _ k' v' =>
-    by_cases h : v = v'
-    . simp [h, denote, addM]
-    . simp [h, denote, addM, ih]
-
-def Monomials.add (m₁ m₂ : Monomials) : Monomials :=
-  match m₂ with
-  | [] => m₁
-  | (k, v) :: m₂ => add (m₁.addM k v) m₂
-
-@[simp] theorem Monomials.denote_add (ctx : Context) (m₁ m₂ : Monomials) : (m₁.add m₂).denote ctx = m₁.denote ctx + m₂.denote ctx := by
-  induction m₂ generalizing m₁ with
-  | nil => simp [add, denote]
-  | cons kv m₂ ih => cases kv with | _ k v =>
-    simp [add, denote, ih]
-
-def Monomials.mul (k : Nat) (m : Monomials) : Monomials :=
-  if k = 0 then
-    []
-  else
-    go m
-where
-  go : Monomials → Monomials
-  | [] => []
-  | (k', v) :: m => (k*k', v) :: go m
-
-@[simp] theorem Monomials.denote_mul (ctx : Context) (k : Nat) (m : Monomials) : (m.mul k).denote ctx = k * m.denote ctx := by
-  simp [mul]
-  by_cases h : k = 0
-  . simp [denote, h]
-  . simp [denote, h]
-    induction m with
-    | nil  => simp [mul.go, denote]
-    | cons kv m ih => cases kv with | _ k' v => simp [mul.go, denote, ih]
-
-def Monomials.insertSorted (k : Nat) (v : Var) (m : Monomials) : Monomials :=
-  match m with
-  | [] => [(k, v)]
-  | (k', v') :: m => if v < v' then (k, v) :: (k', v') :: m else (k', v') :: insertSorted k v m
-
-@[simp] theorem Monomials.denote_insertSorted (ctx : Context) (k : Nat) (v : Var) (m : Monomials) : (m.insertSorted k v).denote ctx = m.denote ctx + k * v.denote ctx := by
-  induction m with
-  | nil => simp [insertSorted, denote]
-  | cons kv m ih => cases kv with | _ k' v' => by_cases h : v < v' <;> simp [h, insertSorted, denote, ih]
-
-def Monomials.sort (m : Monomials) : Monomials :=
-  let rec go (m : Monomials) (r : Monomials) : Monomials :=
-    match m with
-    | [] => r
-    | (k, v) :: m => go m (r.insertSorted k v)
-  go m []
-
-@[simp] theorem Monomials.denote_sort_go (ctx : Context) (m : Monomials) (r : Monomials) : (sort.go m r).denote ctx = m.denote ctx + r.denote ctx := by
-  induction m generalizing r with
-  | nil => simp [sort.go, denote]; done
-  | cons kv m ih => cases kv with | _ k v => simp [sort.go, denote, ih]
-
-@[simp] theorem Monomials.denote_sort (ctx : Context) (m : Monomials) : m.sort.denote ctx = m.denote ctx := by
-  simp [sort, denote]
-
-@[simp] theorem Monomials.denote_append (ctx : Context) (m₁ m₂ : Monomials) : (m₁ ++ m₂).denote ctx = m₁.denote ctx + m₂.denote ctx := by
-  match m₁ with
-  | []  => simp [denote]
-  | (k, v) :: m₁ => simp [denote, denote_append ctx m₁ m₂]
-
-@[simp] theorem Monomials.denote_cons (ctx : Context) (k : Nat) (v : Var) (m : Monomials) : denote ctx ((k, v) :: m) = k * v.denote ctx + m.denote ctx := by
-  match m with
-  | []  => simp [denote]
-  | _ :: m => simp [denote, denote_cons ctx k v m]
-
-@[simp] theorem Monomials.denote_reverseAux (ctx : Context) (m₁ m₂ : Monomials) : denote ctx (List.reverseAux m₁ m₂) = denote ctx (m₁ ++ m₂) := by
-  match m₁ with
-  | [] => simp [denote, List.reverseAux]
-  | (k, v) :: m₁ => simp [denote, List.reverseAux, denote_reverseAux ctx m₁]
-
-@[simp] theorem Monomials.denote_reverse (ctx : Context) (m : Monomials) : denote ctx (List.reverse m) = denote ctx m := by
-  simp [List.reverse]
-
-def Monomials.cancelAux (fuel : Nat) (m₁ m₂ r₁ r₂ : Monomials) : Monomials × Monomials :=
-  match fuel with
-  | 0 => (r₁.reverse ++ m₁, r₂.reverse ++ m₂)
-  | fuel + 1 =>
-    match m₁, m₂ with
-    | m₁, [] => (r₁.reverse ++ m₁, r₂.reverse)
-    | [], m₂ => (r₁.reverse, r₂.reverse ++ m₂)
-    | (k₁, v₁) :: m₁, (k₂, v₂) :: m₂ =>
-      if v₁ < v₂ then
-        cancelAux fuel m₁ ((k₂, v₂) :: m₂) ((k₁, v₁) :: r₁) r₂
-      else if v₁ > v₂ then
-        cancelAux fuel ((k₁, v₁) :: m₁) m₂ r₁ ((k₂, v₂) :: r₂)
-      else if k₁ < k₂ then
-        cancelAux fuel m₁ m₂ r₁ ((k₂ - k₁, v₁) :: r₂)
-      else if k₁ > k₂ then
-        cancelAux fuel m₁ m₂ ((k₁ - k₂, v₁) :: r₁) r₂
-      else
-        cancelAux fuel m₁ m₂ r₁ r₂
-
-def Monomials.denote_eq (ctx : Context) (mp : Monomials × Monomials) : Prop := mp.1.denote ctx = mp.2.denote ctx
-
--- TODO : cleanup proof
-theorem Monomials.denote_cancelAux (ctx : Context) (fuel : Nat) (m₁ m₂ r₁ r₂ : Monomials)
-    (h : denote_eq ctx (r₁.reverse ++ m₁, r₂.reverse ++ m₂)) : denote_eq ctx (cancelAux fuel m₁ m₂ r₁ r₂) := by
-  induction fuel generalizing m₁ m₂ r₁ r₂ with
-  | zero => assumption
-  | succ fuel ih =>
-    simp [cancelAux]
-    split
-    . simp_all
-    . simp_all
-    . rename_i k₁ v₁ m₁ k₂ v₂ m₂
-      by_cases hltv : v₁ < v₂
-      . simp [hltv]; apply ih; simp [denote_eq, denote] at h |-; assumption
-      . by_cases hgtv : v₁ > v₂
-        . simp [hltv, hgtv]; apply ih; simp [denote_eq, denote] at h |-; assumption
-        . simp [hltv, hgtv]
-          have heqv : v₁ = v₂ := Nat.le_antisymm (Nat.ge_of_not_lt hgtv) (Nat.ge_of_not_lt hltv)
-          subst heqv
-          by_cases hltk : k₁ < k₂
-          . simp [hltk]; apply ih; simp [denote_eq, denote] at h |-
-            rw [Nat.mul_sub_right_distrib, ← Nat.add_assoc, ← Nat.add_sub_assoc]
-            apply Eq.symm
-            apply Nat.sub_eq_of_eq_add
-            simp [h]
-            exact Nat.mul_le_mul_right _ (Nat.le_of_lt hltk)
-          . by_cases hgtk : k₁ > k₂
-            . simp [hltk, hgtk]
-              apply ih
-              simp [denote_eq, denote] at h |-
-              rw [Nat.mul_sub_right_distrib, ← Nat.add_assoc, ← Nat.add_sub_assoc]
-              apply Nat.sub_eq_of_eq_add
-              simp [h]
-              exact Nat.mul_le_mul_right _ (Nat.le_of_lt hgtk)
-            . simp [hltk, hgtk]
-              have heqk : k₁ = k₂ := Nat.le_antisymm (Nat.ge_of_not_lt hgtk) (Nat.ge_of_not_lt hltk)
-              subst heqk
-              apply ih
-              simp [denote_eq, denote] at h |-
-              rw [← Nat.add_assoc, ← Nat.add_assoc] at h
-              exact Nat.add_right_cancel h
-
-def Monomials.cancel (m₁ m₂ : Monomials) : Monomials × Monomials :=
-  cancelAux (m₁.length + m₂.length) m₁ m₂ [] []
-
-theorem Monomials.denote_cancel (ctx : Context) (m₁ m₂ : Monomials) (h : denote_eq ctx (m₁, m₂)) : denote_eq ctx (cancel m₁ m₂) := by
-  simp [cancel]
-  apply denote_cancelAux
-  simp [h]
-
-structure Poly where
-  m : Monomials := []
-  k : Nat       := 0
-  deriving Repr
-
-def Poly.denote (ctx : Context) (p : Poly) : Nat :=
-  p.m.denote ctx + p.k
-
-def Poly.addK (p : Poly) (k : Nat) : Poly :=
-  { p with k := p.k + k }
-
-def Poly.addM (p : Poly) (k : Nat) (v : Var) : Poly :=
-  { p with m := p.m.addM k v }
-
-@[simp] theorem Poly.denote_addM (ctx : Context) (p : Poly) (k : Nat) (v : Var) : (p.addM k v).denote ctx = p.denote ctx + k * v.denote ctx := by
-  simp [denote, addM]
-
-def Poly.add (p q : Poly) : Poly :=
-  { m := p.m.add q.m, k := p.k + q.k }
-
-@[simp] theorem Poly.denote_add (ctx : Context) (p q : Poly) : (p.add q).denote ctx = p.denote ctx + q.denote ctx := by
-  simp [add, denote]
-
-def Poly.mul (k : Nat) (p : Poly) : Poly :=
-  { p with m := p.m.mul k, k := p.k * k }
-
-@[simp] theorem Poly.denote_mul (ctx : Context) (k : Nat) (p : Poly) : (p.mul k).denote ctx = k * p.denote ctx := by
-  simp [denote, mul]
-
-def Poly.sort (p : Poly) : Poly :=
-  { p with m := p.m.sort }
-
-@[simp] theorem Poly.denote_sort (ctx : Context) (p : Poly) : p.sort.denote ctx = p.denote ctx := by
-  simp [denote, sort]
-
-def Expr.toPoly : Expr → Poly
-  | Expr.num k    => { k }
-  | Expr.var i    => { m := [(1, i)] }
-  | Expr.add a b  => a.toPoly.add b.toPoly
-  | Expr.mulL k a => a.toPoly.mul k
-  | Expr.mulR a k => a.toPoly.mul k
-
-@[simp] theorem Expr.denote_toPoly (ctx : Context) (e : Expr) : e.toPoly.denote ctx = e.denote ctx := by
-  induction e with
-  | num k => simp [denote, toPoly, Poly.denote, Monomials.denote]
-  | var i => simp [denote, toPoly, Poly.denote, Monomials.denote]
-  | add a b iha ihb => simp [denote, toPoly, iha, ihb]; done
-  | mulL k a ih => simp [denote, toPoly, ih]; done
-  | mulR k a ih => simp [denote, toPoly, ih]; done
-
-theorem Expr.eq_of_toPoly_sort_eq (ctx : Context) (a b : Expr) (h : a.toPoly.sort = b.toPoly.sort) : a.denote ctx = b.denote ctx := by
-  have h := congrArg (Poly.denote ctx) h
-  simp at h
-  assumption
+open Nat.Linear
 
 example (x₁ x₂ x₃ : Nat) : (x₁ + x₂) + (x₂ + x₃) = x₃ + 2*x₂ + x₁ :=
-  Expr.eq_of_toPoly_sort_eq { vars := [x₁, x₂, x₃] }
+  Expr.eq_of_toNormPoly [x₁, x₂, x₃]
    (Expr.add (Expr.add (Expr.var 0) (Expr.var 1)) (Expr.add (Expr.var 1) (Expr.var 2)))
    (Expr.add (Expr.add (Expr.var 2) (Expr.mulL 2 (Expr.var 1))) (Expr.var 0))
    rfl
+
+example (x₁ x₂ x₃ : Nat) : ((x₁ + x₂) + (x₂ + x₃) = x₃ + x₂) = (x₁ + x₂ = 0) :=
+  Expr.of_cancel_eq [x₁, x₂, x₃]
+    (Expr.add (Expr.add (Expr.var 0) (Expr.var 1)) (Expr.add (Expr.var 1) (Expr.var 2)))
+    (Expr.add (Expr.var 2) (Expr.var 1))
+    (Expr.add (Expr.var 0) (Expr.var 1))
+    (Expr.num 0)
+    rfl
+
+example (x₁ x₂ x₃ : Nat) : ((x₁ + x₂) + (x₂ + x₃) ≤ x₃ + x₂) = (x₁ + x₂ ≤ 0) :=
+  Expr.of_cancel_le [x₁, x₂, x₃]
+    (Expr.add (Expr.add (Expr.var 0) (Expr.var 1)) (Expr.add (Expr.var 1) (Expr.var 2)))
+    (Expr.add (Expr.var 2) (Expr.var 1))
+    (Expr.add (Expr.var 0) (Expr.var 1))
+    (Expr.num 0)
+    rfl
+
+example (x₁ x₂ x₃ : Nat) : ((x₁ + x₂) + (x₂ + x₃) < x₃ + x₂) = (x₁ + x₂ < 0) :=
+  Expr.of_cancel_lt [x₁, x₂, x₃]
+    (Expr.add (Expr.add (Expr.var 0) (Expr.var 1)) (Expr.add (Expr.var 1) (Expr.var 2)))
+    (Expr.add (Expr.var 2) (Expr.var 1))
+    (Expr.add (Expr.var 0) (Expr.var 1))
+    (Expr.num 0)
+    rfl
+
+example (x₁ x₂ : Nat) : x₁ + 2 ≤ 3*x₂ → 4*x₂ ≤ 3 + x₁ → 3 ≤ 2*x₂ → False :=
+  Certificate.of_combine_isUnsat [x₁, x₂]
+    [ (1, { eq := false, lhs := Expr.add (Expr.var 0) (Expr.num 2), rhs := Expr.mulL 3 (Expr.var 1) }),
+      (1, { eq := false, lhs := Expr.mulL 4 (Expr.var 1), rhs := Expr.add (Expr.num 3) (Expr.var 0) }),
+      (0, { eq := false, lhs := Expr.num 3, rhs := Expr.mulL 2 (Expr.var 1) }) ]
+    rfl
+
+example (x : Nat) (xs : List Nat) : (sizeOf x < 1 + (1 + sizeOf x + sizeOf xs)) = True :=
+  ExprCnstr.eq_true_of_isValid [sizeOf x, sizeOf xs]
+    { eq := false, lhs := Expr.inc (Expr.var 0), rhs := Expr.add (Expr.num 1) (Expr.add (Expr.add (Expr.num 1) (Expr.var 0)) (Expr.var 1)) }
+    rfl
+
+example (x : Nat) (xs : List Nat) : (1 + (1 + sizeOf x + sizeOf xs) < sizeOf x) = False :=
+  ExprCnstr.eq_false_of_isUnsat [sizeOf x, sizeOf xs]
+    { eq := false, lhs := Expr.inc <| Expr.add (Expr.num 1) (Expr.add (Expr.add (Expr.num 1) (Expr.var 0)) (Expr.var 1)), rhs := Expr.var 0 }
+    rfl
